src/Typing.v
@@ -18,6 +18,7 @@ From ITree Require Import
      ITree
      ITreeFacts
      Basics.MonadState
+     Basics.MonadProp
      Events.State
      Events.Nondeterminism
      Eq.Eq
@@ -30,102 +31,6 @@ From Paco Require Import
 Import ITreeNotations.
 Import CatNotations.
 Import ITree.Basics.Basics.Monads.
-
-Section PropM.
-
-  (* Global Instance EqM_Prop : EqM Ensembles.Ensemble := Ensembles.Same_set. *)
-
-  (* Global Instance Functor_Prop : Functor.Functor Ensembles.Ensemble := *)
-  (*   {| fmap := fun _ _ f Pa b => exists a, Pa a /\ f a = b |}. *)
-
-  (* Global Instance Monad_Prop : Monad Ensembles.Ensemble := *)
-  (*   {| *)
-  (*   ret := fun _ x y => x = y; *)
-  (*   bind := fun _ _ Pa K b => exists a, In _ Pa a /\ In _ (K a) b *)
-  (*   |}. *)
-
-  (* Lemma bind_ret_l_Prop : forall A B (f : A -> Ensembles.Ensemble B) a, *)
-  (*     eqm (bind (ret a) f) (f a). *)
-  (* Proof. *)
-  (*   split; repeat intro; simpl in *. *)
-  (*   - destruct H as (? & ? & ?). red in H. subst; auto. *)
-  (*   - eexists; split; eauto. reflexivity. *)
-  (* Qed. *)
-
-  (* Lemma bind_ret_r_Prop : forall (A : Type) (Pa : Ensembles.Ensemble A), *)
-  (*     eqm (bind Pa (fun a => ret a)) Pa. *)
-  (* Proof. *)
-  (*   split. repeat intro; simpl in *. *)
-  (*   - destruct H as (? & ? & ?). red in H0; subst; auto. *)
-  (*   - red. repeat intro. eexists; split; eauto. reflexivity. *)
-  (* Qed. *)
-
-  (* Lemma bind_bind_Prop : *)
-  (*   forall A B C (Pa : Ensembles.Ensemble A) *)
-  (*     (f : A -> Ensembles.Ensemble B) (g : B -> Ensembles.Ensemble C), *)
-  (*     eqm (bind (bind Pa f) g) (bind Pa (fun y => bind (f y) g)). *)
-  (* Proof. *)
-  (*   intros. split; repeat intro; simpl in *; *)
-  (*             [destruct H as (? & (? & ? & ?) & ?) | destruct H as (? & ? & (? & ? & ?))]; *)
-  (*             do 2 (eexists; split; eauto). *)
-  (* Qed. *)
-
-  Definition PropM (T : Type) (R : Type) := Ensembles.Ensemble (T * R).
-
-  Global Instance EqM_PropM T : EqM (PropM T) := fun _ => Ensembles.Same_set _.
-
-  Global Instance Functor_PropM T : Functor.Functor (PropM T) :=
-    {|
-    fmap := fun A B (f : A -> B) (Pa : PropM T A) (pb : T * B) =>
-              exists (pa : T * A), Pa pa /\ (fst pa, f (snd pa)) = pb
-    |}.
-
-  Global Instance Monad_PropM T : Monad (PropM T) :=
-    {|
-    ret := fun A a pa => a = snd pa;
-    bind := fun A B (Pa : PropM T A) (K : A -> PropM T B) (pb : T * B) =>
-              exists (a : A), In _ Pa (fst pb, a) /\ In _ (K a) pb
-    |}.
-
-  Lemma bind_ret_l_PropM : forall T A B (f : A -> PropM T B) a,
-      eqm (bind (ret a) f) (f a).
-  Proof.
-    split; repeat intro; simpl in *.
-    - destruct H as (? & ? & ?). red in H. subst. auto.
-    - exists a; split; [split |]; auto.
-  Qed.
-
-  Lemma bind_ret_r_PropM : forall T (A : Type) (Pa : PropM T A),
-      eqm (bind Pa (fun a => ret a)) Pa.
-  Proof.
-    split; repeat intro; simpl in *.
-    - destruct H as (? & ? & ?). red in H0. destruct x; subst; auto.
-    - exists (snd x); split; auto; destruct x; red; auto.
-  Qed.
-
-  Lemma bind_bind_PropM :
-    forall T A B C (Pa : PropM T A)
-      (f : A -> PropM T B) (g : B -> PropM T C),
-      eqm (bind (bind Pa f) g) (bind Pa (fun y => bind (f y) g)).
-  Proof.
-    intros. split; repeat intro; simpl in *;
-              [destruct H as (? & (? & ? & ?) & ?) | destruct H as (? & ? & (? & ? & ?))];
-              do 2 (eexists; split; eauto).
-  Qed.
-
-  Instance MonadLaws_PropM T : @MonadLaws (PropM T) _ _.
-  Proof.
-    constructor; [apply bind_ret_l_PropM | apply bind_ret_r_PropM | apply bind_bind_PropM |].
-    repeat intro. (* TODO: clean up this case *)
-    destruct H.
-    split; repeat red; repeat intro.
-    - repeat red in H2. decompose [ex and] H2; clear H2.
-      exists x2. split; auto. apply H0; auto.
-    - repeat red in H2. decompose [ex and] H2; clear H2.
-      exists x2. split; auto. apply H0; auto.
-  Qed.
-
-End PropM.
 
 Definition sep_step p q : Prop :=
   forall r, p ⊥ r -> q ⊥ r.
@@ -175,117 +80,20 @@ Proof.
   - symmetry. auto.
 Qed.
 
-Section MonadIter.
-  (* should probably give this a shorter name later *)
-  Variant iter_stateT_PropM_perm_gen
-          {X I : Type}
-          iter'
-          (step : I -> config -> (PropM perm (config * (I + X))))
-          (i : I)
-          (c : config)
-          (pcr : perm * (config * X))
-  : Prop :=
-  | iter_done :
-      let p := fst pcr in
-      let c' := fst (snd pcr) in
-      let r := snd (snd pcr) in
-      (* dom p c -> *) (* for a ret, any perm should be fine. *)
-      step i c (p, (c', inr r)) ->
-      iter_stateT_PropM_perm_gen iter' step i c pcr
-  | iter_step :
-      let p := fst pcr in
-      let c'' := fst (snd pcr) in
-      let r := snd (snd pcr) in
-      (* dom p c -> *)
-      (* exists i' c', step i c (p, (c' (inl i'))) /\ *)
-
-      (forall i' c',
-                dom p c ->
-                step i c (p, (c', (inl i'))) ->
-                upd p c c' /\ (* needs to be here rather than in the handlers, since this is not a precondition *)
-                (* as a result, we don't actually need to give the handlers access to the perm anymore *)
-                (exists p', sep_step p p' /\
-                       dom p' c' /\
-                       iter' step i' c' (p', (c'', r)))) ->
-      iter_stateT_PropM_perm_gen iter' step i c pcr.
-
-  Definition iter_stateT_PropM_perm {R I : Type} step i c pcr : Prop :=
-    paco4 (@iter_stateT_PropM_perm_gen R I) bot4 step i c pcr.
-
-  Lemma iter_stateT_PropM_perm_gen_mon X I : monotone4 (@iter_stateT_PropM_perm_gen X I).
-  Proof.
-    repeat intro.
-    destruct x3 as (? & ? & ?).
-    inversion IN.
-    - constructor. auto.
-    - econstructor 2; intros; eauto. simpl in *.
-      edestruct H; eauto.
-      split; auto. decompose [ex and] H3; clear H3; eauto.
-  Qed.
-  Hint Resolve iter_stateT_PropM_perm_gen_mon : paco.
-
-  (* CoInductive iter_stateT_PropM_perm *)
-  (*             {R I : Type} *)
-  (*             (step : I -> config -> (PropM perm (config * (I + R)))) *)
-  (*             (i : I) *)
-  (*             (c : config) *)
-  (*             (pcr : perm * (config * R)) *)
-  (*   : Prop := *)
-  (* | iter_done : *)
-  (*     let p := fst pcr in *)
-  (*     let c' := fst (snd pcr) in *)
-  (*     let r := snd (snd pcr) in *)
-  (*     (* dom p c -> *) (* for a ret, any perm should be fine. *) *)
-  (*     step i c (p, (c', inr r)) -> *)
-  (*     iter_stateT_PropM_perm step i c pcr *)
-  (* | iter_step : *)
-  (*     let p := fst pcr in *)
-  (*     let c'' := fst (snd pcr) in *)
-  (*     let r := snd (snd pcr) in *)
-  (*     (forall i' c', dom p c -> *)
-  (*               step i c (p, (c', (inl i'))) -> *)
-  (*               upd p c c' /\ (* needs to be here rather than in the handlers, since this is not a precondition *) *)
-  (*               (* as a result, we don't actually need to give the handlers access to the perm anymore *) *)
-  (*               (exists p', sep_step p p' /\ *)
-  (*                      dom p' c' /\ *)
-  (*                      iter_stateT_PropM_perm step i' c' (p', (c'', r)))) -> *)
-  (*     iter_stateT_PropM_perm step i c pcr. *)
-
-  Global Instance MonadIter_stateT' : MonadIter (stateT config (PropM perm)) :=
-    @iter_stateT_PropM_perm.
-
-  (* CoInductive iter_PropM_perm {R I : Type} (step : I -> PropM perm (I + R)) (i : I) (pr : perm * R) *)
-  (*   : Prop := *)
-  (* | iter_done *)
-  (*   : step i (fst pr, (inr (snd pr))) -> iter_PropM_perm step i pr *)
-  (* | iter_step i' *)
-  (*   : let p := fst pr in *)
-  (*     let r := snd pr in *)
-  (*     step i (p, (inl i')) -> *)
-  (*     (exists p', sep_step p p' /\ *)
-  (*            iter_PropM_perm step i' (p', r)) -> *)
-  (*     iter_PropM_perm step i pr *)
-  (* . *)
-  (* Global Instance MonadIter_PropM : MonadIter (PropM perm) := @iter_PropM_perm. *)
-
-  (** Iter Laws **)
-  Global Instance IterUnfold_TODO : IterUnfold (Kleisli (stateT config (PropM perm))) sum.
-  Proof.
-    repeat intro. split; repeat intro.
-    - destruct x as (? & ? & ?). red in H.
-      pinversion H; simpl in *.
-      + replace p0 with p in *; auto. replace c' with c in *; auto.
-        replace r with b0 in *; auto. clear p0 c' r.
-        eexists; split; eauto. repeat red; auto.
-      + replace p0 with p in *; auto. replace c'' with c in *; auto.
-        replace r with b0 in *; auto. clear p0 c'' r.
-        Abort.
-
-End MonadIter.
-
 Section ts.
+  Variant MemoryE : Type -> Type :=
+  | Load : forall (p : SByte), MemoryE SByte
+  | Store : forall (p v : SByte) , MemoryE unit
+  .
 
-  Definition E := (stateE config +' nondetE).
+  (* Definition h_memory : MemoryE ~> stateE config := *)
+  (*   fun R e => *)
+  (*     match e with *)
+  (*     | Store p v => Put *)
+  (*     @Get _. *)
+
+  (* Definition E := (stateE config +' nondetE). *)
+  Definition E := (MemoryE +' nondetE).
 
   Context {R : Type}.
 
@@ -327,8 +135,12 @@ Section ts.
   | step_tau : forall t c, step (Tau t) c t c
   | step_nondet_true : forall k c, step (vis Or k) c (k true) c
   | step_nondet_false : forall k c, step (vis Or k) c (k false) c
-  | step_get : forall k c, step (vis (Get _) k) c (k c) c
-  | step_put : forall k c c', step (vis (Put _ c') k) c (k tt) c'
+  | step_load : forall k c p v, read c p = Some v ->
+                           step (vis (Load (Ptr p)) k) c (k v) c
+  | step_store : forall k c c' p v, write c p v = Some c' ->
+                               step (vis (Store (Ptr p) v) k) c (k tt) c'
+  (* | step_get : forall k c, step (vis (Get _) k) c (k c) c *)
+  (* | step_put : forall k c c', step (vis (Put _ c') k) c (k tt) c' *)
   .
 
   Lemma step_bind : forall (t1 t2 : itree E R) (c1 c2 : config) (k : R -> itree E R),
@@ -342,10 +154,12 @@ Section ts.
       apply bisimulation_is_eq in bind_vis. rewrite bind_vis. constructor.
     - pose proof (bind_vis _ _ (subevent _ Or) k0 k) as bind_vis.
       apply bisimulation_is_eq in bind_vis. rewrite bind_vis. constructor.
-    - pose proof (bind_vis _ _ (subevent _ (Get _)) k0 k) as bind_vis.
-      apply bisimulation_is_eq in bind_vis. rewrite bind_vis. constructor.
-    - pose proof (bind_vis _ _ (subevent _ (Put _ c2)) k0 k) as bind_vis.
-      apply bisimulation_is_eq in bind_vis. rewrite bind_vis. constructor.
+    - pose proof (bind_vis _ _ (subevent _ (Load (Ptr p))) k0 k) as bind_vis.
+      apply bisimulation_is_eq in bind_vis. rewrite bind_vis.
+      (* constructor doesn't work here for some reason *)
+      apply (step_load (fun v => x <- k0 v;; k x) _ _ _ H0).
+    - pose proof (bind_vis _ _ (subevent _ (Store (Ptr p) v)) k0 k) as bind_vis.
+      apply bisimulation_is_eq in bind_vis. rewrite bind_vis. constructor; auto.
   Qed.
 
   Lemma step_ret_bind : forall (t1 t2 : itree E R) (c1 c2 : config) (r : R),
@@ -362,94 +176,19 @@ Section ts.
       exists t'', step (par t1 t') c t'' c /\ step t'' c (par t2 t') c'.
   Proof.
     inversion 1; subst;
-      (rewrite rewrite_par; unfold par_match; simpl; repeat eexists; constructor).
+      try (rewrite rewrite_par; unfold par_match; simpl; repeat eexists; constructor; auto).
+    (* as above, load case needs its constructor manually applied... *)
+    rewrite rewrite_par; unfold par_match; simpl; repeat eexists. constructor.
+    apply (step_load (fun x => par (k x) t') _ _ _ H0).
   Qed.
   Lemma par_step_right : forall (t1 t2 t' : itree E R) (c c' : config),
       step t1 c t2 c' ->
       exists t'', step (par t' t1) c t'' c /\ step t'' c (par t' t2) c'.
   Proof.
     inversion 1; subst;
-      (rewrite rewrite_par; unfold par_match; simpl; repeat eexists; constructor).
-  Qed.
-
-  Definition h_nondet : nondetE ~> stateT config (PropM perm) :=
-    fun R e c =>
-      fun (pcr : perm * (config * R)) =>
-        let p := fst pcr in
-        let c' := fst (snd pcr) in
-        let r := snd (snd pcr) in
-        c = c' /\
-        match e in (nondetE bool) return bool -> Prop with
-        | Or => fun r => r = true \/ r = false
-        end r.
-
-  Definition h_state : stateE config ~> stateT config (PropM perm) :=
-    fun R e c =>
-      fun (pcr : perm * (config * R)) =>
-        let p := fst pcr in
-        let c' := fst (snd pcr) in
-        let r := snd (snd pcr) in
-        match e in (stateE _ X) return X -> Prop with
-        | Get _ => fun r => c' = c /\ r = c
-        | Put _ c'' => fun r => c' = c'' /\
-                              r = tt
-        end r.
-
-  Lemma h_nondet_perm X e c p q x :
-    h_nondet X e c (p, x) -> h_nondet X e c (q, x).
-  Proof.
-    intros. destruct e; simpl in *; auto.
-  Qed.
-  Lemma h_state_perm X e c p q x :
-    h_state X e c (p, x) -> h_state X e c (q, x).
-  Proof.
-    intros. destruct e; simpl in *; auto.
-  Qed.
-
-  Definition handler : E ~> stateT config (PropM perm) := case_ h_state h_nondet.
-
-  Definition empty_config := Build_config nil.
-
-  Lemma type_interp_ret :
-    forall p c (r : R) (Hdom: dom p c), interp handler (Ret r) c (p, (c, r)).
-  Proof.
-    intros. repeat red. pstep. constructor; auto.
-    cbn; auto.
-  Qed.
-
-  Lemma type_interp_lte :
-    forall p q (t : itree E R) c r,
-      interp handler t c (p, (c, r)) -> p <= q -> interp handler t c (q, (c, r)).
-  Proof.
-    intros. pinversion H; auto.
-    - simpl in p0, c', r. replace p0 with p in *; auto. replace c' with c in *; auto.
-      replace r0 with r in *; auto. clear p0 c' r0.
-      pstep. constructor.
-      destruct (observe t0); simpl in *; auto.
-      decompose [ex and] H1; clear H1. inversion H4.
-    - simpl in p0, c'', r0. replace p0 with p in *; auto. replace c'' with c in *; auto.
-      replace r0 with r in *; auto. clear p0 c'' r0.
-      pstep. constructor 2; intros.
-      edestruct H1; clear H1.
-      + apply H0; auto.
-      + destruct (observe t0); simpl in *; inversion H3; clear H3; subst; auto.
-        destruct x as (? & ? & ?). decompose [and] H1; clear H1. simpl in *.
-        inversion H4; clear H4; subst. exists (p, (c', x)). split; simpl; auto.
-        destruct e; [apply (h_state_perm _ _ _ p) | apply (h_nondet_perm _ _ _ p)]; auto.
-      + split; simpl; [apply H0; auto |].
-        decompose [ex and] H5; clear H5. exists x. split; [| split]; auto.
-        eapply sep_step_lte; eauto.
-    - apply iter_stateT_PropM_perm_gen_mon. (* TODO automation *)
-  Qed.
-
-  Lemma type_interp_spin :
-    forall p c n (Hdom: dom p c),
-      interp handler (ITree.spin : itree E R) c (p, (c, n)).
-  Proof.
-    Set Printing All. pcofix CIH. Unset Printing All.
-    pstep. econstructor 2; intros.
-    rewrite rewrite_spin in H0. inversion H0; subst.
-    split; intuition. exists p. split; [| split]; simpl; intuition.
+      try (rewrite rewrite_par; unfold par_match; simpl; repeat eexists; constructor; auto).
+    rewrite rewrite_par; unfold par_match; simpl; repeat eexists. constructor 3.
+    apply (step_load (fun x => par t' (k x)) _ _ _ H0).
   Qed.
 
   Variant typing_perm_gen typing (p : perm) (t : itree E R) : Prop :=
@@ -551,21 +290,21 @@ Section ts.
         + split; [| split]; auto.
       - symmetry in Heqi. pose proof (bisimulation_is_eq _ _ (simpobs Heqi)) as Heqi'.
         rewrite Heqi' in Ht1.
-        destruct e; [destruct s | destruct n]; pinversion Ht1; exists (p1 * p2);
+        destruct e; [destruct m | destruct n]; pinversion Ht1; exists (p1 * p2);
           (split; intuition; [| split; [| split]]; auto);
           left; pstep; constructor; intros ? [Hdom1' [Hdom2' Hsep']] ? ? Hstep;
             inversion Hstep; auto_inj_pair2; subst.
-        + destruct (H _ Hdom1' _ _ (step_get _ _)) as [? [p [? [? ?]]]]. pclearbot.
+        + destruct (H _ Hdom1' _ _ (step_load _ _ _ _ H5)) as [? [p [? [? ?]]]]. pclearbot.
           split; intuition.
           exists (p * p2). split; [| split]; auto.
           * apply sep_step_sep_conj_l; auto.
           * split; [| split]; auto.
-        + destruct (H _ Hdom1' _ _ (step_put _ _ _)) as [? [p [? [? ?]]]]. pclearbot.
+        + destruct (H _ Hdom1' _ _ (step_store _ _ _ _ _ H6)) as [? [p [? [? ?]]]]. pclearbot.
           split; [constructor |]; auto.
           exists (p * p2). split; [| split]; auto.
           * apply sep_step_sep_conj_l; auto.
           * split; [| split]; auto.
-            eapply dom_respects. apply Hsep'. apply H0. auto.
+          eapply dom_respects. apply Hsep'. apply H0. auto.
         + destruct (H _ Hdom1' _ _ (step_nondet_true _ _)) as [? [p [? [? ?]]]]. pclearbot.
           split; intuition.
           exists (p * p2). split; [| split]; auto.
@@ -590,16 +329,16 @@ Section ts.
         + split; [| split]; auto. symmetry. apply H2; auto.
       - symmetry in Heqi. pose proof (bisimulation_is_eq _ _ (simpobs Heqi)) as Heqi'.
         rewrite Heqi' in Ht2. symmetry in Hsep.
-        destruct e; [destruct s | destruct n]; pinversion Ht2; exists (p1 * p2);
+        destruct e; [destruct m | destruct n]; pinversion Ht2; exists (p1 * p2);
           (split; intuition; [| split; [| split]]; auto);
           left; pstep; constructor; intros ? [Hdom1' [Hdom2' Hsep']] ? ? Hstep;
             inversion Hstep; auto_inj_pair2; subst; symmetry in Hsep.
-        + destruct (H _ Hdom2' _ _ (step_get _ _)) as [? [p [? [? ?]]]]. pclearbot.
+        + destruct (H _ Hdom2' _ _ (step_load _ _ _ _ H5)) as [? [p [? [? ?]]]]. pclearbot.
           split; intuition.
           exists (p1 * p). split; [| split]; auto.
           * apply sep_step_sep_conj_r; auto.
           * split; [| split]; auto. symmetry. apply H2; auto.
-        + destruct (H _ Hdom2' _ _ (step_put _ _ _)) as [? [p [? [? ?]]]]. pclearbot.
+        + destruct (H _ Hdom2' _ _ (step_store _ _ _ _ _ H6)) as [? [p [? [? ?]]]]. pclearbot.
           split; [constructor |]; auto.
           exists (p1 * p). split; [| split]; auto.
           * apply sep_step_sep_conj_r; auto.
@@ -630,15 +369,3 @@ Section ts.
     specialize (Ht2 _ H0). eapply typing_perm_lte; eauto. eapply parallel_perm; eauto.
   Qed.
 End ts.
-
-Definition test : itree (stateE config +' _) unit :=
-  par
-    (x <- (trigger (Get _)) ;; (trigger (Put _ x)))
-    (par (vis (Get _) (fun x => Ret tt))
-         (Ret tt)).
-
-(* Compute (burn 10 test). *)
-
-(* Eval cbv in (burn 10 (step (trigger (Put _ 0)) 1)). *)
-(* Eval cbn in (burn 10 (step test 1)). *)
-(* Eval cbn in (burn 10 (run_state test 1)). *)
